try separating typ and type

use_typinf.ml
@@ -23,6 +23,10 @@ let rec list_of_coqlist = function
     Nil -> []
   | Cons (a, l) -> a::list_of_coqlist l;;
 
+let rec coqlist_of_list = function
+    [] -> Nil
+  | a :: l -> Cons (a, coqlist_of_list l);;
+
 let typinf1 trm =
   match typinf' trm with
     Some (Pair (kenv, typ)) ->
@@ -31,33 +35,33 @@ let typinf1 trm =
 
 open Typinf.Cstr;;
 
+let rec nat_of_int n = if n <= 0 then O else S (nat_of_int (n-1));;
+
+let app a b = Coq_trm_app (a,b)
+let abs a = Coq_trm_abs a
+let var n = Variables.var_of_nat (nat_of_int n)
+let bvar n = Coq_trm_bvar (nat_of_int n)
+let matches l =
+  Coq_trm_cst (Const.Coq_matches (coqlist_of_list l))
+let tag v =
+  Coq_trm_cst (Const.Coq_tag v);;
+
 (* First example: (Coq_tag A) is a function constant, which takes any value
    and returns a polymorphic variant A with this value as argument *)
 (* This example is equivalent to the ocaml term [fun x -> `A0 x] *)
-typinf1 (Coq_trm_cst (Const.Coq_tag (Variables.var_of_nat O)));;
-
-let rec nat_of_int n = if n <= 0 then O else S (nat_of_int (n-1));;
+typinf1 (tag (var 0));;
 
 (* Second example: (Coq_matches [A1; ..; An]) is a n+1-ary function constant
    which takes n functions and a polymorphic variant as argument, and
    (fi v) if the argument was (Ai v). *)
 (* This example is equivalent to [function `A20 x -> x | `A21 x -> x] *)
 let mtch f1 f2 =
-  Coq_trm_app (Coq_trm_app (
-    Coq_trm_cst
-      (Const.Coq_matches
-         (Cons (Variables.var_of_nat (nat_of_int 20),
-                Cons (Variables.var_of_nat (nat_of_int 21), Nil)))),
-               f1),
-               f2);;
-let trm = mtch (Coq_trm_abs (Coq_trm_bvar O)) (Coq_trm_abs (Coq_trm_bvar O));;
+  app (app (matches [var 20; var 21]) f1) f2
+let trm = mtch (abs (bvar 0)) (abs (bvar 0));;
 typinf1 trm;;
 
 (* Another example, producing a recursive type *)
 (* OCaml equivalent: [fun x -> match x with `A20 y -> y | `A21 y -> x] *)
-let trm2 =
-  Coq_trm_abs
-    (Coq_trm_app
-       (mtch (Coq_trm_abs (Coq_trm_bvar O)) (Coq_trm_abs (Coq_trm_bvar (S O))),
-        Coq_trm_bvar O));;
+let trm2' =
+  abs (app (mtch (abs (bvar 0)) (abs (bvar 1))) (bvar 0)) ;;
 typinf1 trm2;;
